src/study/Nemonuri.Study.CSharpSyntaxRewriter2.Modifier2/Nemonuri.StratifiedNodes.Common.fst
@@ -3,3 +3,25 @@ module Nemonuri.StratifiedNodes.Common
 //--- type definitions ---
 let aggregator (t:Type) = (aggregated:t) -> (aggregating:t) -> t
 //---|
+
+//--- theory members ---
+// https://learn.microsoft.com/en-us/dotnet/api/system.linq.enumerable.skipwhile?view=net-9.0
+let rec skip_while #t
+  (l:list t) 
+  (predicate:t -> Tot bool)
+  : Tot (list t) (decreases l) =
+  match l with
+  | [] -> []
+  | hd::tl ->
+    match (predicate hd) with
+    | true -> l
+    | false -> skip_while tl predicate
+
+// https://learn.microsoft.com/en-us/dotnet/api/system.linq.enumerable.takewhile?view=net-9.0
+(*
+let rec take_while #t
+  (l:list t) 
+  (predicate:t -> Tot bool)
+  : Tot (list t) (decreases l) =
+*)
+//---|
