src/study/Nemonuri.Study.CSharpSyntaxRewriter2.Modifier2/Nemonuri.StratifiedNodes.Walkers.fst
@@ -17,15 +17,15 @@ let rec walk #t #t2
   (child_parent_aggregator:Common.aggregator t2) 
   (left_right_aggregator:Common.aggregator t2)
   (continue_predicate:N.node t -> t2 -> bool)
-  (ancestors:C.ancestor_list t) //{ if L.isEmpty ancestor_list then true else C.is_child (L.last ancestor_list) node }
+  (ancestors:C.next_head_given_ancestor_list node)
   : Tot t2 (decreases (node.level)) =
-  let v1 = selector ancestors node in
+  let v1 = selector node ancestors in
   if (N.is_leaf node) || (not (continue_predicate node v1)) then
     v1
   else
-    let next_ancestors = (node::ancestors) in
+    let next_ancestors = C.concatenate_as_ancestor_list node ancestors in
     C.select_and_aggregate_from_children
-      node (fun ancestors child -> 
+      node (fun child ancestors -> 
         (walk child selector child_parent_aggregator left_right_aggregator continue_predicate ancestors)
       ) child_parent_aggregator left_right_aggregator continue_predicate next_ancestors v1
 //---|
